proof checker fixes and refactors

logic.v
@@ -38,14 +38,22 @@ Fixpoint member (f:formula) (C:context) : Prop :=
     | p::rest => if formula_dec f p then True else member f rest
   end.
 
+Print sumor.
+
+Definition subst_p (p:pcpl) (prin: principal) (n:var) : principal :=
+  match prin with 
+    | Pcpl_p _ => prin
+    | Var_p v =>
+      match lt_eq_lt_dec v n with
+       | inleft (left _ ) => Var_p v
+       | inleft (right _ ) => Pcpl_p p
+       | inright _ => Var_p (v-1)
+      end
+  end.
+
 Fixpoint subst (a:pcpl) (f:formula) (n:var) : formula :=
   match f with
-    | Pred_f s (Var_p v) => if eq_nat_dec v n 
-                              then Pred_f s (Pcpl_p a)
-                              else if gt_dec v n
-                                then Pred_f s (Var_p (v -1))
-                                else Pred_f s (Var_p v)
-    | Pred_f s (Pcpl_p p) => Pred_f s (Pcpl_p p)
+    | Pred_f s v => Pred_f s (subst_p a v n) (* TODO fix the rest *)
     | Impl_f f1 f2 => Impl_f (subst a f1 n) (subst a f2 n)
     | Signed_f (Var_p v) f => if eq_nat_dec v n
                                 then Signed_f (Pcpl_p a) (subst a f n)
@@ -68,13 +76,15 @@ Fixpoint subst (a:pcpl) (f:formula) (n:var) : formula :=
     | Abs_f f => Abs_f (subst a f (n+1))
   end.
 
+Definition env := list (option pcpl).
+
 Reserved Notation "c '|--' g" (at level 70).
 
 Inductive entails : context -> formula -> Prop :=
 | Init_e : forall C f, member f C -> C |-- f
 | Tauto_e : forall C f, C |-- f -> 
                 forall a, C |-- Says_f a f
-| Weaken_e : forall C f1 f2, f1::C |-- f2 -> 
+| Weaken_Impl_e : forall C f1 f2, f1::C |-- f2 -> 
                                    C |-- Impl_f f1 f2
 | Impl_e : forall C f1 f2 f3, C |-- f1 -> 
                                   f2::C |-- f3 ->
@@ -87,6 +97,7 @@ Inductive entails : context -> formula -> Prop :=
                                  (Says_f a f1)::C |-- Says_f a f2
 | Spec_e : forall C p f1 f2 a, (subst p f1 0)::C |-- Says_f a f2 ->
                                  (Abs_f f1)::C |-- Says_f a f2
+| Weaken_e : forall f1 C f2, C |-- f2 -> f1::C |-- f2
 where "C '|--' F" := (entails C F).
 
 Definition delegate a b p := Signed_f (Pcpl_p a) (Abs_f (Impl_f (Says_f (Pcpl_p b) (Pred_f p (Var_p 0))) (Pred_f p (Var_p 0)))).
@@ -100,7 +111,7 @@ Ltac prove_auth :=
     | [ |- (Confirms_f ?a _)::_ |-- Says_f ?a _ ] => eapply Confirms_e
     | [ |- (Signed_f ?a _)::_ |-- Says_f ?a _ ] => eapply Signed_e
     | [ |- (Impl_f _ _)::_ |-- _ ] => eapply Impl_e
-    | [ |- _ |-- Impl_f _ _ ] => eapply Weaken_e
+    | [ |- _ |-- Impl_f _ _ ] => eapply Weaken_Impl_e
     | [ |- _ |-- Says_f _ _ ] => eapply Tauto_e
     | [ |- _ |-- _] => try (econstructor ; simpl ; auto)
   end.
@@ -148,54 +159,223 @@ match p with
   | Says_Spec_r f _ _ _ => f
 end.
 
-Fixpoint check (g:formula) (p:proof) : Prop :=
-  (* if g = proof_goal p ... else False *)
+
+Definition prsubst (p:principal) (e:env) : principal :=
   match p with
-    | Signed_r f => match f with
-                      | Signed_f _ _ => if formula_dec f g then True else False
-                      | _ => False
-                    end
-    | Confirms_r f => match f with
-                      | Confirms_f _ _ => if formula_dec f g then True else False
-                      | _ => False
-                      end
-    | Tauto_r f p1 => match f with
-                        | Says_f _ f2 => if formula_dec f g then check f2 p1 else False
-                        | _ => False
-                      end
-    | Impl_r f p1 p2 p3 => match proof_goal p2 with
-                             | Impl_f f1 f2 => check f1 p1 /\ check (Impl_f f1 f2) p2 /\ check (Impl_f f2 f) p3
-                             | _ => False
-                           end
-    | Says_Confirms_r f p1 p2 => match f with
-                                   | Says_f a f2 => match proof_goal p1 with
-                                                      | Confirms_f a f1 => check (Confirms_f a f1) p1 /\ check (Impl_f f1 f) p2
-                                                      | _ => False
-                                                    end
-                                   | _ => False
-                                 end
-    | Says_Signed_r f p1 p2 => match f with
-                                   | Says_f a f2 => match proof_goal p1 with
-                                                      | Signed_f a f1 => check (Signed_f a f1) p1 /\ check (Impl_f f1 f) p2
-                                                      | _ => False
-                                                    end
-                                   | _ => False
-                                 end
-    | Says_Says_r f p1 p2 =>  match f with
-                                   | Says_f a f2 => match proof_goal p1 with
-                                                      | Says_f a f1 => check (Says_f a f1) p1 /\ check (Impl_f f1 f) p2
-                                                      | _ => False
-                                                    end
-                                   | _ => False
-                                 end
-    | Says_Spec_r f theP p1 p2 => match f with
+    | Pcpl_p thep => p
+    | Var_p v => match nth_error e v with
+                   | Some (Some prl) => (Pcpl_p prl)
+                   | Some (None) => p
+                   | None => p
+                 end
+  end.
+
+Fixpoint subst_simul (e:env) (f:formula) : formula :=
+  match f with
+    | Pred_f s v => Pred_f s (prsubst v e) (* TODO fix the rest *)
+    | Impl_f f1 f2 => Impl_f (subst_simul e f1) (subst_simul e f2)
+    | Signed_f p f => Signed_f (prsubst p e) (subst_simul e f)
+    | Says_f p f => Says_f (prsubst p e) (subst_simul e f)
+    | Confirms_f p f => Confirms_f (prsubst p e) (subst_simul e f) 
+    | Abs_f f => Abs_f (subst_simul (None::e) f)
+  end.
+
+Fixpoint formula_comp e1 f1 e2 f2 : option (subst_simul e1 f1 = subst_simul e2 f2).
+  refine (
+  match f1, f2 with
+    | Pred_f p1 pr1, Pred_f p2 pr2 => 
+      if string_dec p1 p2 
+        then let p1 := prsubst pr1 e1 in
+             let p2 := prsubst pr2 e2 in
+               if principal_dec p1 p2 then Some _ else None
+        else None
+    | Impl_f f3 f4, Impl_f f5 f6 => 
+      if formula_comp e1 f3 e2 f5 then if formula_comp e1 f4 e2 f6 then Some _ else None else None
+    | Signed_f pr1 f3, Signed_f pr2 f4 => 
+      let p1 := prsubst pr1 e1 in
+        let p2 := prsubst pr2 e2 in
+          if principal_dec p1 p2 then 
+            if formula_comp e1 f3 e2 f4 then Some _ else None else None
+    | Says_f pr1 f3, Says_f pr2 f4 => 
+      let p1 := prsubst pr1 e1 in
+        let p2 := prsubst pr2 e2 in
+          if principal_dec p1 p2 then 
+            if formula_comp e1 f3 e2 f4 then Some _ else None else None
+    | Confirms_f pr1 f3, Confirms_f pr2 f4 => 
+      let p1 := prsubst pr1 e1 in
+        let p2 := prsubst pr2 e2 in
+          if principal_dec p1 p2 then 
+            if formula_comp e1 f3 e2 f4 then Some _ else None else None
+    | Abs_f f3, Abs_f f4 =>
+      if formula_comp (None::e1) f3 (None::e2) f4 then Some _ else None
+    | _ , _=> None
+  end); clear formula_comp ; try abstract ( subst; 
+  simpl; repeat match goal with 
+                  | [ H : _ = _ |- _ ] => rewrite H
+                end; reflexivity).
+Defined.
+
+Fixpoint axioms (e:env) (p:proof) : context :=
+match p with
+  | Signed_r f => (subst_simul e f)::nil
+  | Confirms_r f => (subst_simul e f)::nil
+  | Tauto_r f p1 => axioms e p1
+  | Impl_r f p1 p2 p3 => List.app (axioms e p1) (List.app (axioms e p2) (axioms e p3))
+  | Says_Confirms_r f p1 p2 => List.app (axioms e p1) (axioms e p2) 
+  | Says_Signed_r f p1 p2 => List.app (axioms e p1) (axioms e p2)
+  | Says_Says_r f p1 p2 => List.app (axioms e p1) (axioms e p2)
+  | Says_Spec_r f a p1 p2 => List.app (axioms ((Some a)::e) p1) (axioms ((Some a)::e) p2)
+end.
+
+Fixpoint all_none (e:env) : Prop :=
+  match e with
+    | nil => True
+    | None::e2 => all_none e2
+    | _ => False
+  end.
+
+Lemma nth_foo : forall T ls n (x:T), nth_error ls n = Some x -> In x ls.
+Admitted.
+
+Lemma prsubst_nil : forall p e, all_none e -> ((prsubst p e) = p).
+Proof.
+  intros.
+  unfold prsubst.
+  destruct p ; auto.
+  case_eq (nth_error e v) ; intros ; subst ; auto.
+  destruct o ; auto.
+  elimtype False.
+  apply nth_foo in H0.
+  induction e.
+  auto.
+  destruct H0.
+  subst ; simpl in * ; congruence.
+  apply IHe. simpl in H. destruct a ; auto ; exfalso ; auto.
+  apply H0.
+Qed.
+
+Lemma subst_nil : forall f e, all_none e -> ((subst_simul e f) = f).
+Proof.
+  induction f ; intros ; simpl ; try(rewrite prsubst_nil ; auto) ;
+  simpl ; auto ; try(rewrite IHf) ; auto ;
+  specialize (IHf1 e H) ; specialize (IHf2 e H) ; rewrite IHf1 ; rewrite IHf2 ; auto.
+Qed.
+
+(** Proof checker - Checks the proof tree from the bottom up. *)
+Fixpoint check (g:formula) (e:env) (p:proof) : option (axioms e p |-- subst_simul e g).
+  refine (
+    let f := proof_goal p in
+  match formula_comp e g e f with
+    | None => None
+    | Some fg_eq =>
+      match p with
+        | Signed_r (Signed_f pr f1) => if formula_comp e f e (Signed_f pr f1) then Some _ else None
+        | Confirms_r (Confirms_f pr f1) => if formula_comp e f e (Confirms_f pr f1) then Some _ else None
+        | Tauto_r (Says_f pr f1) p1 => if formula_comp e f e (Says_f pr f1) then if check f1 e p1 then Some _ else None else None
+        | Impl_r f3 p1 p2 p3 => if formula_comp e f e f3
+                                  then match proof_goal p2 with
+                                         | Impl_f f1 f2 => if check f1 e p1
+                                                             then if check (Impl_f f1 f2) e p2
+                                                                    then if check (Impl_f f2 f3) e p3 then Some _ else None
+                                                                    else None
+                                                             else None
+                                         | _ => None
+                                       end
+                                  else None
+        | _ => None
+      end
+  end) ;
+  simpl ; rewrite fg_eq ; rewrite _H ; try(simpl ; apply Init_e ; unfold member ; destruct formula_dec ; auto ; fail).
+  simpl ; apply Tauto_e ; auto.
+  simpl in *. 
+
+Lemma weaken_ctxt : forall f1 f2 C1 C2, C1 |-- f1 -> In f2 C1 -> In f2 C2 -> C2 |-- f1.
+Admitted.
+
+Lemma weaken_ctxt_app : forall f1 C1 C2, C1 |-- f1 -> (C1++C2)%list |-- f1.
+Admitted.
+
+Lemma app_impl : forall ax1 ax2 f1 f2, ax1 |-- Impl_f f1 f2 -> ax2 |-- f1 -> List.app ax1 ax2 |-- f2.
+Proof.
+  intros.
+  assert ((ax1 ++ ax2)%list |-- Impl_f f1 f2).
+  apply weaken_ctxt_app ; auto.
+  assert ((ax1 ++ ax2)%list |-- f1).
+  apply weaken_ctxt_app ; auto.
+
+
+Lemma rep_ax : forall f1 f2 f3 C, f1::C |-- f2 -> f3::nil |-- f1 -> f3::C |-- f2.
+Proof.
+  intros.
+  
+  
+  
+  assert (f3::C |-- f1).
+  eapply weaken_ctxt ; auto.
+  clear H0.
+  apply (Impl_e 
+
+Show.
+  
+
+  simpl in *.  induction p1. induction p2. induction p3. simpl in *.
+  apply Weaken_e in _H0.
+  apply Weaken_e in _H1.
+
+  Show.
+Defined.
+
+
+rewrite subst_nil in fg_eq ; rewrite subst_nil in fg_eq.
+  rewrite fg_eq.
+  
+
+(*
+        | Confirms_r f => match f with
+                            | Confirms_f _ _ => formula_comp e g e f
+                            | _ => False
+                          end
+        | Tauto_r f p1 => match f with
+                            | Says_f _ f2 => match formula_comp e g e f with 
+                                               | True => check f2 e p1 
+                                             end
+                            | _ => False
+                          end
+        | Impl_r f p1 p2 p3 => match proof_goal p2 with
+                                 | Impl_f f1 f2 => check f1 e p1 /\ check (Impl_f f1 f2) e p2 /\ check (Impl_f f2 f) e p3
+                                 | _ => False
+                               end
+        | Says_Confirms_r f p1 p2 => match f with
+                                       | Says_f a f2 => match proof_goal p1 with
+                                                          | Confirms_f a f1 => check (Confirms_f a f1) e p1 /\ check (Impl_f f1 f) e p2
+                                                          | _ => False
+                                                        end
+                                       | _ => False
+                                     end
+        | Says_Signed_r f p1 p2 => match f with
+                                     | Says_f a f2 => match proof_goal p1 with
+                                                        | Signed_f a f1 => check (Signed_f a f1) e p1 /\ check (Impl_f f1 f) e p2
+                                                        | _ => False
+                                                      end
+                                     | _ => False
+                                   end
+        | Says_Says_r f p1 p2 =>  match f with
                                     | Says_f a f2 => match proof_goal p1 with
-                                                       | Abs_f f1 => check (Abs_f f1) p1 /\ check (Impl_f (subst theP f1 0) f) p2
+                                                       | Says_f a f1 => check (Says_f a f1) e p1 /\ check (Impl_f f1 f) e p2
                                                        | _ => False
                                                      end
                                     | _ => False
                                   end
-  end.
+        | Says_Spec_r f theP p1 p2 => match f with
+                                        | Says_f a f2 => match proof_goal p1 with
+                                                           | Abs_f f1 => check (Abs_f f1) e p1 /\ check (Impl_f (subst theP f1 0) f) e p2
+                                                           | _ => False
+                                                         end
+                                        | _ => False
+                                      end
+      end
+   end. (* The formula does not match the goal *)*)
+
 
 Fixpoint axioms (p:proof) : context :=
 match p with
@@ -211,14 +391,20 @@ end.
 
 (** Prove that check f p -> (all signed or confirmed things) |- f *)
 
-Lemma foo : forall f1 f2, (if formula_dec f1 f2 then True else False) = (if formula_dec f2 f1 then True else False). 
+(*Lemma foo : forall f1 f2, (if formula_dec f1 f2 then True else False) = (if formula_dec f2 f1 then True else False). 
 Proof.
   intros ; destruct formula_dec ; destruct formula_dec ; simpl ; congruence.
 Qed.  
 
-Theorem checker_correct : forall f p, check f p -> axioms p |-- f.
+Theorem checker_correct : forall f e p, check f e p -> axioms p |-- f.
 Proof.
   intros.
+  induction p.
+  simpl in *.
+  destruct f0 ; try (exfalso ; auto ; fail).
+  
+  
+
   induction p ; try (simpl in * ; destruct f0 ; try (exfalso ; auto ; fail) ; prove_auth ; try (rewrite foo ; auto) ; fail).
   assert (axioms (Tauto_r f0 p) = axioms p).
   simpl ; auto.
@@ -227,4 +413,4 @@ Proof.
   destruct f0 ; try (exfalso ; auto ; fail).
   destruct formula_dec.
   rewrite e in H0.
-Admitted.
+Admitted.*)
